\section{Optimal Betting Fraction}
\label{section:optimal-betting-fraction}

\begin{theorem}
\label{theo:opt_beta}
Assume that the function $\phi(z)=F_t(x+z)$, is piece-wise logarithmically convex in $[-\infty,0)$ and $(0,\infty]$. Then, for any $z\in \R$, we have
\[
\argmin_{\beta} \max_{|g_t|\leq 1} \ \frac{F_t(x+g_t)}{1 + \beta g_t} =\frac{F_t(x+1) - F_t(x-1)}{F_t(x+1) + F_t(x-1)}~.
\]
\end{theorem}
\begin{proof}
First consider the case that $g_t=0$. In this case, $\frac{F_t(x+g_t)}{1 + \beta g_t}=F_t(x)$, independently of $\beta$. Hence, in the following we can exclude the case $g_t=0$.

Minimizing $\frac{\phi(z)}{1+\beta z}$ is equivalent to minimize the function $g(z,\beta)$ defined as
\[
g(z,\beta) := \ln \phi(z) - \log(1+\beta z)~.
\]
We have that $g(z,\beta)$ is piece-wise convex on $[-\infty,0)$ and $(0,\infty]$, w.r.t. the first argument.
Hence, the maximum of $g(z,\beta)$ is attained in $z=-1$ or $z=1$, given that the case $z=0$ is escluded by assumption.
Hence, we want to choose $\beta$ as
\[
\argmin_{\beta} \max_{z \in \{-1, 1\}} \ g(z,\beta),
\]
in other words we want to set $\beta$ such that $g(1)=g(-1)$, that is
\[
\beta^* = \frac{\exp\left(\ln \phi(1) - \ln \phi(-1)\right)-1}{\exp\left(\ln \phi(1) - \ln \phi(-1)\right)+1}
= \frac{\phi(1) - \phi(-1)}{\phi(1) + \phi(-1)}~.
\]
\end{proof}
