\section{Properties of KT}

\begin{theorem}[KT potential]
\label{theorem:kt-potential}
Let $\delta \ge 0$. The sequence of functions $\{F_t\}_{t=0}^\infty$, $F_t:(-t-\delta-1, t+\delta+1) \to \R_+$
defined by
$$
F_t(x) = \frac{2^t \Gamma(\delta + 1) \Gamma(\frac{t+\delta+1}{2} + \frac{x}{2}) \Gamma(\frac{t+\delta+1}{2} - \frac{x}{2})}{\Gamma(\frac{\delta+1}{2})^2 \Gamma(T+\delta+1)} \; .
$$
is a sequence of excellent coin-betting potentials.
Futhermore, for any $x \in (-t-\delta-1, t+\delta+1)$,
$$
\frac{F_t(x+1) - F_{t}(x-1)}{F_t(x+1) + F_{t}(x-1)} = \frac{x}{t+\delta} \; .
$$
\end{theorem}

\begin{proof}
Property (1) of definition of coin-betting potential is satified, since
$$
F_0(0) = \epsilon \frac{\Gamma(\frac{1}{2}) \Gamma(\frac{1}{2})}{\pi} = \epsilon \; ,
$$
where we used that $\Gamma(\frac{1}{2}) = \pi$. $F_t$ is clearly even.
Since $\lim_{x \to 0^+} \Gamma(x) = +\infty$ and $\Gamma(\frac{t+1}{2})$,
$\lim_{x \to \frac{t+1}{2}^+} F_t(x) = \lim_{x \to -\frac{t+1}{2}} F_t(x) = \infty$.
Bohr-Mollerup theorem states that $\Gamma(x)$ is logaritmically convex
on $(0,\infty)$. Therefore $F_t$ is logaritmically convex as well.
The fact that $F_t$ is increasing on $[0,\frac{t+1}{2})$ is proved
in the Appendix as Lemma~\ref{lemma:???}. This establishes property (2).
Property (3) can be verified by direct calculation
$$
TODO
$$

We now verify that KT estimator $\beta_t$ defined by \eqref{equation:kt-estimator}
satisfies \eqref{equation:potential-based-strategy}. Indeed, let $x=\sum_{i=1}^{t-1} g_i$
\begin{align*}
\frac{F_t(\sum_{i=1}^{t-1} g_i + 1) - F_t(\sum_{i=1}^{t-1} g_i - 1)}{F_t(\sum_{i=1}^{t-1} g_i + 1) + F_t(\sum_{i=1}^{t-1} g_i - 1)}
& = \frac{F_t(x + 1) - F_t(x - 1)}{F_t(x + 1) + F_t(x - 1)} \\
& = \frac{\Gamma(\frac{t+2}{2} + \frac{x}{2}) \Gamma(\frac{t}{2} - \frac{x}{2}) - \Gamma(\frac{t}{2} + \frac{x}{2}) \Gamma(\frac{t+2}{2} - \frac{x}{2})}{\Gamma(\frac{t+2}{2} + \frac{x}{2}) \Gamma(\frac{t}{2} - \frac{x}{2}) + \Gamma(\frac{t}{2} + \frac{x}{2}) \Gamma(\frac{t+2}{2} - \frac{x}{2})} \\
& = \frac{(\frac{t}{2} + \frac{x}{2})\Gamma(\frac{t}{2} + \frac{x}{2}) \Gamma(\frac{t}{2} - \frac{x}{2}) - (\frac{t}{2} - \frac{x}{2})\Gamma(\frac{t}{2} + \frac{x}{2}) \Gamma(\frac{t}{2} - \frac{x}{2})}{(\frac{t}{2} + \frac{x}{2})\Gamma(\frac{t}{2} + \frac{x}{2}) \Gamma(\frac{t}{2} - \frac{x}{2}) + (\frac{t}{2} - \frac{x}{2})\Gamma(\frac{t}{2} + \frac{x}{2}) \Gamma(\frac{t}{2} - \frac{x}{2})} \\
& = \frac{(\frac{t}{2} + \frac{x}{2}) - (\frac{t}{2} - \frac{x}{2})}{(\frac{t}{2} + \frac{x}{2}) + (\frac{t}{2} - \frac{x}{2})} \\
& = \frac{x}{t} \\
& = \beta_t
\end{align*}
\end{proof}
